fix(F*): more proofs tweaks to Spec.Intrinsics.fst

libcrux-ml-dsa/proofs/fstar/spec/Spec.Intrinsics.fsti
@@ -776,17 +776,18 @@ val i32_bit_zero_lemma_to_positive vec
   : Lemma (requires forall i. v i % 32 == 31 ==> vec.(i) == Core_models.Abstractions.Bit.Bit_Zero)
           (ensures forall i. v (to_i32x8 vec i) >= 0)
 
+#push-options "--z3rlimit 80"
 let rewrite_eq_sub_mod (#t: inttype {signed t}) (a b c: int_t t)
   : Lemma (requires v a > minint t /\ a == b `sub_mod_opaque` c)
           (ensures  neg a `add_mod_opaque` b == c)
           = reveal_opaque_arithmetic_ops #t
+#pop-options
 
 val to_i32x8_eq_to_bv_eq (a b: bv256)
   : Lemma (requires forall i. to_i32x8 a i == to_i32x8 b i)
           (ensures a == b)
 
-let lemma_from_i32x8_def_pt f: Lemma (forall i. to_i32x8 (from_i32x8 (FStar.FunctionalExtensionality.on (n:u64{v n < 8}) f)) i == f i)
-  = admit ()
+val lemma_from_i32x8_def_pt (f: (i:u64{v i < 8}) -> i32): Lemma (forall i. to_i32x8 (from_i32x8 (FStar.FunctionalExtensionality.on (i:u64{v i < 8}) f)) i == f i)
 
 let mk_i32x8 (f: (i:u64{v i < 8}) -> i32): r: bv256 {forall i. to_i32x8 r i == f i}
  = lemma_from_i32x8_def_pt f;
